src/cbor/pulse/raw/everparse/CBOR.Pulse.Raw.EverParse.Nondet.Compare.ArrayCase.fsti
@@ -1,0 +1,55 @@
+module CBOR.Pulse.Raw.EverParse.Nondet.Compare.ArrayCase
+#lang-pulse
+include CBOR.Pulse.Raw.EverParse.Nondet.Compare.Base
+open CBOR.Spec.Util
+open CBOR.Spec.Raw.EverParse
+open CBOR.Pulse.Raw.EverParse.Type
+open CBOR.Pulse.Raw.EverParse.Match
+open CBOR.Pulse.Raw.EverParse.Match.Fuel
+open CBOR.Pulse.Raw.EverParse.Access
+open CBOR.Pulse.Raw.EverParse.Read
+open Pulse.Lib.Pervasives
+open Pulse.Lib.Trade
+
+module SZ = FStar.SizeT
+module R = Pulse.Lib.Reference
+module Trade = Pulse.Lib.Trade.Util
+module I = LowParse.PulseParse.Iterator
+module IT = LowParse.PulseParse.Iterator.Type
+module NG = CBOR.Pulse.Raw.EverParse.Nondet.Gen
+
+inline_for_extraction
+val compare_cbor_raw_array_case_fuel
+  (#data_model: Ghost.erased (raw_data_item -> raw_data_item -> bool))
+  (f64: squash SZ.fits_u64)
+  (map_bound: option SZ.t)
+  (n: Ghost.erased nat { Ghost.reveal n >= 1 })
+  (compare_rec: compare_cbor_raw_fuel_t data_model (NG.option_sz_v map_bound) (Ghost.hide (Ghost.reveal n - 1)))
+  (x1: cbor_raw)
+  (x2: cbor_raw)
+  (len: SZ.t)
+  (_: squash (
+    CBOR_Case_Array? x1 /\ CBOR_Case_Array? x2 /\
+    IT.mixed_list_length (CBOR_Case_Array?.v x1).cbor_array_ptr == len /\
+    IT.mixed_list_length (CBOR_Case_Array?.v x2).cbor_array_ptr == len
+  ))
+  (#pm1: perm)
+  (#v1: Ghost.erased raw_data_item)
+  (#pm2: perm)
+  (#v2: Ghost.erased raw_data_item)
+: stt (option bool)
+    (cbor_raw_match_fuel n pm1 x1 v1 **
+     cbor_raw_match_fuel n pm2 x2 v2 **
+     pure (
+       Array? (Ghost.reveal v1) /\ Array? (Ghost.reveal v2) /\
+       List.Tot.length (Array?.v (Ghost.reveal v1)) == SZ.v len /\
+       List.Tot.length (Array?.v (Ghost.reveal v2)) == SZ.v len /\
+       raw_data_item_size v1 <= Ghost.reveal n /\
+       raw_data_item_size v2 <= Ghost.reveal n /\
+       check_equiv data_model (NG.option_sz_v map_bound) v1 v2 ==
+         check_equiv_list (Array?.v (Ghost.reveal v1)) (Array?.v (Ghost.reveal v2)) (check_equiv_map data_model (NG.option_sz_v map_bound))
+     ))
+    (fun res ->
+      cbor_raw_match_fuel n pm1 x1 v1 **
+      cbor_raw_match_fuel n pm2 x2 v2 **
+      pure (res == check_equiv data_model (NG.option_sz_v map_bound) v1 v2))
