src/cbor/pulse/raw/everparse/CBOR.Pulse.Raw.EverParse.Nondet.Compare.BasicMap.fst
@@ -1,0 +1,272 @@
+module CBOR.Pulse.Raw.EverParse.Nondet.Compare.BasicMap
+#lang-pulse
+include CBOR.Pulse.Raw.EverParse.Nondet.Compare.ListForAll
+open CBOR.Spec.Util
+open CBOR.Spec.Raw.EverParse
+open CBOR.Pulse.Raw.EverParse.Type
+open CBOR.Pulse.Raw.EverParse.Match
+open CBOR.Pulse.Raw.EverParse.Match.Fuel
+open CBOR.Pulse.Raw.EverParse.MapEntry.Fuel
+open CBOR.Pulse.Raw.EverParse.Access
+open LowParse.Spec.Combinators
+open Pulse.Lib.Pervasives
+open Pulse.Lib.Trade
+
+module SZ = FStar.SizeT
+module Trade = Pulse.Lib.Trade.Util
+module I = LowParse.PulseParse.Iterator
+module NG = CBOR.Pulse.Raw.EverParse.Nondet.Gen
+
+#push-options "--z3rlimit 512 --fuel 4 --ifuel 4 --split_queries always"
+
+inline_for_extraction
+```pulse
+fn compare_cbor_raw_basic_fuel_map_case
+  (f64: squash SZ.fits_u64)
+  (map_bound: option SZ.t)
+  (n: Ghost.erased nat { Ghost.reveal n >= 1 })
+  (compare_rec_map: compare_cbor_raw_fuel_t basic_data_model (option_nat_decrement_safe (NG.option_sz_v map_bound)) (Ghost.hide (Ghost.reveal n - 1)))
+  (x1 x2: cbor_raw)
+  (#pm1: perm) (#v1: Ghost.erased raw_data_item)
+  (#pm2: perm) (#v2: Ghost.erased raw_data_item)
+requires
+  cbor_raw_match_fuel n pm1 x1 v1 **
+  cbor_raw_match_fuel n pm2 x2 v2 **
+  pure (Map? (Ghost.reveal v1) /\ Map? (Ghost.reveal v2) /\
+        raw_data_item_size v1 <= Ghost.reveal n /\
+        raw_data_item_size v2 <= Ghost.reveal n)
+returns res: option bool
+ensures
+  cbor_raw_match_fuel n pm1 x1 v1 **
+  cbor_raw_match_fuel n pm2 x2 v2 **
+  pure (res == check_equiv_map_total basic_data_model (NG.option_sz_v map_bound) v1 v2)
+{
+  cbor_raw_match_fuel_eq_succ n pm1 x1 v1;
+  cbor_raw_match_fuel_eq_succ n pm2 x2 v2;
+  rewrite (cbor_raw_match_fuel n pm1 x1 v1)
+       as (cbor_raw_match_aux parse_raw_data_item (cbor_raw_match_fuel (n - 1)) pm1 x1 v1);
+  rewrite (cbor_raw_match_fuel n pm2 x2 v2)
+       as (cbor_raw_match_aux parse_raw_data_item (cbor_raw_match_fuel (n - 1)) pm2 x2 v2);
+  raw_data_item_size_eq v1;
+  raw_data_item_size_eq v2;
+  cbor_raw_match_aux_cases (cbor_raw_match_fuel (n - 1)) pm1 x1;
+  cbor_raw_match_aux_cases (cbor_raw_match_fuel (n - 1)) pm2 x2;
+  cbor_raw_match_aux_fields (cbor_raw_match_fuel (n - 1)) pm1 x1;
+  cbor_raw_match_aux_fields (cbor_raw_match_fuel (n - 1)) pm2 x2;
+  check_equiv_map_map_eq basic_data_model (NG.option_sz_v map_bound) (Ghost.reveal v1) (Ghost.reveal v2) () ();
+  match map_bound {
+    Some mb_v -> {
+      if (mb_v = 0sz) {
+        cbor_raw_match_fuel_eq_succ n pm1 x1 v1;
+        cbor_raw_match_fuel_eq_succ n pm2 x2 v2;
+        rewrite (cbor_raw_match_aux parse_raw_data_item (cbor_raw_match_fuel (n - 1)) pm1 x1 v1)
+             as (cbor_raw_match_fuel n pm1 x1 v1);
+        rewrite (cbor_raw_match_aux parse_raw_data_item (cbor_raw_match_fuel (n - 1)) pm2 x2 v2)
+             as (cbor_raw_match_fuel n pm2 x2 v2);
+        None #bool
+      } else {
+        option_nat_decrement_safe_spec (NG.option_sz_v map_bound);
+        let map_ml1 = cbor_raw_get_map_aux (cbor_raw_match_fuel (n - 1)) pm1 x1 ();
+        with pm1_m map1_entries . assert (
+          I.mixed_list_match (fun (pm0: perm) (elem: cbor_map_entry cbor_raw) (v: (raw_data_item & raw_data_item)) -> cbor_map_entry_match (cbor_raw_match_fuel (n - 1)) pm0 elem v) (nondep_then parse_raw_data_item parse_raw_data_item) pm1_m map_ml1 map1_entries **
+          Trade.trade
+            (I.mixed_list_match (fun (pm0: perm) (elem: cbor_map_entry cbor_raw) (v: (raw_data_item & raw_data_item)) -> cbor_map_entry_match (cbor_raw_match_fuel (n - 1)) pm0 elem v) (nondep_then parse_raw_data_item parse_raw_data_item) pm1_m map_ml1 map1_entries)
+            (cbor_raw_match_aux parse_raw_data_item (cbor_raw_match_fuel (n - 1)) pm1 x1 v1)
+        );
+        rewrite
+          (I.mixed_list_match (fun (pm0: perm) (elem: cbor_map_entry cbor_raw) (v: (raw_data_item & raw_data_item)) -> cbor_map_entry_match (cbor_raw_match_fuel (n - 1)) pm0 elem v) (nondep_then parse_raw_data_item parse_raw_data_item) pm1_m map_ml1 map1_entries)
+          as (I.mixed_list_match (cbor_map_entry_vmatch_fuel (n - 1)) (nondep_then parse_raw_data_item parse_raw_data_item) pm1_m map_ml1 map1_entries);
+        rewrite
+          (Trade.trade
+            (I.mixed_list_match (fun (pm0: perm) (elem: cbor_map_entry cbor_raw) (v: (raw_data_item & raw_data_item)) -> cbor_map_entry_match (cbor_raw_match_fuel (n - 1)) pm0 elem v) (nondep_then parse_raw_data_item parse_raw_data_item) pm1_m map_ml1 map1_entries)
+            (cbor_raw_match_aux parse_raw_data_item (cbor_raw_match_fuel (n - 1)) pm1 x1 v1))
+          as (Trade.trade
+            (I.mixed_list_match (cbor_map_entry_vmatch_fuel (n - 1)) (nondep_then parse_raw_data_item parse_raw_data_item) pm1_m map_ml1 map1_entries)
+            (cbor_raw_match_aux parse_raw_data_item (cbor_raw_match_fuel (n - 1)) pm1 x1 v1));
+        intro
+          (trade
+            (cbor_raw_match_aux parse_raw_data_item (cbor_raw_match_fuel (n - 1)) pm1 x1 v1)
+            (cbor_raw_match_fuel n pm1 x1 v1))
+          #emp
+          fn _ {
+            cbor_raw_match_fuel_eq_succ n pm1 x1 v1;
+            rewrite (cbor_raw_match_aux parse_raw_data_item (cbor_raw_match_fuel (n - 1)) pm1 x1 v1)
+                 as (cbor_raw_match_fuel n pm1 x1 v1)
+          };
+        Trade.trans
+          (I.mixed_list_match (cbor_map_entry_vmatch_fuel (n - 1)) (nondep_then parse_raw_data_item parse_raw_data_item) pm1_m map_ml1 map1_entries)
+          (cbor_raw_match_aux parse_raw_data_item (cbor_raw_match_fuel (n - 1)) pm1 x1 v1)
+          (cbor_raw_match_fuel n pm1 x1 v1);
+        let map_ml2 = cbor_raw_get_map_aux (cbor_raw_match_fuel (n - 1)) pm2 x2 ();
+        with pm2_m map2_entries . assert (
+          I.mixed_list_match (fun (pm0: perm) (elem: cbor_map_entry cbor_raw) (v: (raw_data_item & raw_data_item)) -> cbor_map_entry_match (cbor_raw_match_fuel (n - 1)) pm0 elem v) (nondep_then parse_raw_data_item parse_raw_data_item) pm2_m map_ml2 map2_entries **
+          Trade.trade
+            (I.mixed_list_match (fun (pm0: perm) (elem: cbor_map_entry cbor_raw) (v: (raw_data_item & raw_data_item)) -> cbor_map_entry_match (cbor_raw_match_fuel (n - 1)) pm0 elem v) (nondep_then parse_raw_data_item parse_raw_data_item) pm2_m map_ml2 map2_entries)
+            (cbor_raw_match_aux parse_raw_data_item (cbor_raw_match_fuel (n - 1)) pm2 x2 v2)
+        );
+        rewrite
+          (I.mixed_list_match (fun (pm0: perm) (elem: cbor_map_entry cbor_raw) (v: (raw_data_item & raw_data_item)) -> cbor_map_entry_match (cbor_raw_match_fuel (n - 1)) pm0 elem v) (nondep_then parse_raw_data_item parse_raw_data_item) pm2_m map_ml2 map2_entries)
+          as (I.mixed_list_match (cbor_map_entry_vmatch_fuel (n - 1)) (nondep_then parse_raw_data_item parse_raw_data_item) pm2_m map_ml2 map2_entries);
+        rewrite
+          (Trade.trade
+            (I.mixed_list_match (fun (pm0: perm) (elem: cbor_map_entry cbor_raw) (v: (raw_data_item & raw_data_item)) -> cbor_map_entry_match (cbor_raw_match_fuel (n - 1)) pm0 elem v) (nondep_then parse_raw_data_item parse_raw_data_item) pm2_m map_ml2 map2_entries)
+            (cbor_raw_match_aux parse_raw_data_item (cbor_raw_match_fuel (n - 1)) pm2 x2 v2))
+          as (Trade.trade
+            (I.mixed_list_match (cbor_map_entry_vmatch_fuel (n - 1)) (nondep_then parse_raw_data_item parse_raw_data_item) pm2_m map_ml2 map2_entries)
+            (cbor_raw_match_aux parse_raw_data_item (cbor_raw_match_fuel (n - 1)) pm2 x2 v2));
+        intro
+          (trade
+            (cbor_raw_match_aux parse_raw_data_item (cbor_raw_match_fuel (n - 1)) pm2 x2 v2)
+            (cbor_raw_match_fuel n pm2 x2 v2))
+          #emp
+          fn _ {
+            cbor_raw_match_fuel_eq_succ n pm2 x2 v2;
+            rewrite (cbor_raw_match_aux parse_raw_data_item (cbor_raw_match_fuel (n - 1)) pm2 x2 v2)
+                 as (cbor_raw_match_fuel n pm2 x2 v2)
+          };
+        Trade.trans
+          (I.mixed_list_match (cbor_map_entry_vmatch_fuel (n - 1)) (nondep_then parse_raw_data_item parse_raw_data_item) pm2_m map_ml2 map2_entries)
+          (cbor_raw_match_aux parse_raw_data_item (cbor_raw_match_fuel (n - 1)) pm2 x2 v2)
+          (cbor_raw_match_fuel n pm2 x2 v2);
+        let fwd = compare_cbor_raw_list_for_all_fuel (Ghost.hide (Ghost.reveal n - 1))
+                    #(check_equiv basic_data_model (option_nat_decrement_safe (NG.option_sz_v map_bound)))
+                    compare_rec_map f64
+                    map_ml2 map_ml1;
+        check_equiv_map_list_for_all_ext basic_data_model (option_nat_decrement_safe (NG.option_sz_v map_bound))
+          (list_sum (pair_sum raw_data_item_size raw_data_item_size) (Map?.v (Ghost.reveal v1)) + list_sum (pair_sum raw_data_item_size raw_data_item_size) (Map?.v (Ghost.reveal v2)))
+          (Ghost.reveal map2_entries) (Ghost.reveal map1_entries);
+        match fwd {
+          Some fwd_b -> {
+            if fwd_b {
+              let bwd = compare_cbor_raw_list_for_all_fuel (Ghost.hide (Ghost.reveal n - 1))
+                          #(check_equiv basic_data_model (option_nat_decrement_safe (NG.option_sz_v map_bound)))
+                          compare_rec_map f64
+                          map_ml1 map_ml2;
+              check_equiv_map_list_for_all_ext basic_data_model (option_nat_decrement_safe (NG.option_sz_v map_bound))
+                (list_sum (pair_sum raw_data_item_size raw_data_item_size) (Map?.v (Ghost.reveal v1)) + list_sum (pair_sum raw_data_item_size raw_data_item_size) (Map?.v (Ghost.reveal v2)))
+                (Ghost.reveal map1_entries) (Ghost.reveal map2_entries);
+              Trade.elim _ (cbor_raw_match_fuel n pm1 x1 v1);
+              Trade.elim _ (cbor_raw_match_fuel n pm2 x2 v2);
+              check_equiv_map_eq basic_data_model (NG.option_sz_v map_bound) (Ghost.reveal v1) (Ghost.reveal v2);
+              bwd
+            } else {
+              Trade.elim _ (cbor_raw_match_fuel n pm1 x1 v1);
+              Trade.elim _ (cbor_raw_match_fuel n pm2 x2 v2);
+              check_equiv_map_eq basic_data_model (NG.option_sz_v map_bound) (Ghost.reveal v1) (Ghost.reveal v2);
+              Some false
+            }
+          }
+          None -> {
+            Trade.elim _ (cbor_raw_match_fuel n pm1 x1 v1);
+            Trade.elim _ (cbor_raw_match_fuel n pm2 x2 v2);
+            check_equiv_map_eq basic_data_model (NG.option_sz_v map_bound) (Ghost.reveal v1) (Ghost.reveal v2);
+            None #bool
+          }
+        }
+      }
+    }
+    None -> {
+      option_nat_decrement_safe_spec (NG.option_sz_v map_bound);
+      let map_ml1 = cbor_raw_get_map_aux (cbor_raw_match_fuel (n - 1)) pm1 x1 ();
+      with pm1_m map1_entries . assert (
+        I.mixed_list_match (fun (pm0: perm) (elem: cbor_map_entry cbor_raw) (v: (raw_data_item & raw_data_item)) -> cbor_map_entry_match (cbor_raw_match_fuel (n - 1)) pm0 elem v) (nondep_then parse_raw_data_item parse_raw_data_item) pm1_m map_ml1 map1_entries **
+        Trade.trade
+          (I.mixed_list_match (fun (pm0: perm) (elem: cbor_map_entry cbor_raw) (v: (raw_data_item & raw_data_item)) -> cbor_map_entry_match (cbor_raw_match_fuel (n - 1)) pm0 elem v) (nondep_then parse_raw_data_item parse_raw_data_item) pm1_m map_ml1 map1_entries)
+          (cbor_raw_match_aux parse_raw_data_item (cbor_raw_match_fuel (n - 1)) pm1 x1 v1)
+      );
+      rewrite
+        (I.mixed_list_match (fun (pm0: perm) (elem: cbor_map_entry cbor_raw) (v: (raw_data_item & raw_data_item)) -> cbor_map_entry_match (cbor_raw_match_fuel (n - 1)) pm0 elem v) (nondep_then parse_raw_data_item parse_raw_data_item) pm1_m map_ml1 map1_entries)
+        as (I.mixed_list_match (cbor_map_entry_vmatch_fuel (n - 1)) (nondep_then parse_raw_data_item parse_raw_data_item) pm1_m map_ml1 map1_entries);
+      rewrite
+        (Trade.trade
+          (I.mixed_list_match (fun (pm0: perm) (elem: cbor_map_entry cbor_raw) (v: (raw_data_item & raw_data_item)) -> cbor_map_entry_match (cbor_raw_match_fuel (n - 1)) pm0 elem v) (nondep_then parse_raw_data_item parse_raw_data_item) pm1_m map_ml1 map1_entries)
+          (cbor_raw_match_aux parse_raw_data_item (cbor_raw_match_fuel (n - 1)) pm1 x1 v1))
+        as (Trade.trade
+          (I.mixed_list_match (cbor_map_entry_vmatch_fuel (n - 1)) (nondep_then parse_raw_data_item parse_raw_data_item) pm1_m map_ml1 map1_entries)
+          (cbor_raw_match_aux parse_raw_data_item (cbor_raw_match_fuel (n - 1)) pm1 x1 v1));
+      intro
+        (trade
+          (cbor_raw_match_aux parse_raw_data_item (cbor_raw_match_fuel (n - 1)) pm1 x1 v1)
+          (cbor_raw_match_fuel n pm1 x1 v1))
+        #emp
+        fn _ {
+          cbor_raw_match_fuel_eq_succ n pm1 x1 v1;
+          rewrite (cbor_raw_match_aux parse_raw_data_item (cbor_raw_match_fuel (n - 1)) pm1 x1 v1)
+               as (cbor_raw_match_fuel n pm1 x1 v1)
+        };
+      Trade.trans
+        (I.mixed_list_match (cbor_map_entry_vmatch_fuel (n - 1)) (nondep_then parse_raw_data_item parse_raw_data_item) pm1_m map_ml1 map1_entries)
+        (cbor_raw_match_aux parse_raw_data_item (cbor_raw_match_fuel (n - 1)) pm1 x1 v1)
+        (cbor_raw_match_fuel n pm1 x1 v1);
+      let map_ml2 = cbor_raw_get_map_aux (cbor_raw_match_fuel (n - 1)) pm2 x2 ();
+      with pm2_m map2_entries . assert (
+        I.mixed_list_match (fun (pm0: perm) (elem: cbor_map_entry cbor_raw) (v: (raw_data_item & raw_data_item)) -> cbor_map_entry_match (cbor_raw_match_fuel (n - 1)) pm0 elem v) (nondep_then parse_raw_data_item parse_raw_data_item) pm2_m map_ml2 map2_entries **
+        Trade.trade
+          (I.mixed_list_match (fun (pm0: perm) (elem: cbor_map_entry cbor_raw) (v: (raw_data_item & raw_data_item)) -> cbor_map_entry_match (cbor_raw_match_fuel (n - 1)) pm0 elem v) (nondep_then parse_raw_data_item parse_raw_data_item) pm2_m map_ml2 map2_entries)
+          (cbor_raw_match_aux parse_raw_data_item (cbor_raw_match_fuel (n - 1)) pm2 x2 v2)
+      );
+      rewrite
+        (I.mixed_list_match (fun (pm0: perm) (elem: cbor_map_entry cbor_raw) (v: (raw_data_item & raw_data_item)) -> cbor_map_entry_match (cbor_raw_match_fuel (n - 1)) pm0 elem v) (nondep_then parse_raw_data_item parse_raw_data_item) pm2_m map_ml2 map2_entries)
+        as (I.mixed_list_match (cbor_map_entry_vmatch_fuel (n - 1)) (nondep_then parse_raw_data_item parse_raw_data_item) pm2_m map_ml2 map2_entries);
+      rewrite
+        (Trade.trade
+          (I.mixed_list_match (fun (pm0: perm) (elem: cbor_map_entry cbor_raw) (v: (raw_data_item & raw_data_item)) -> cbor_map_entry_match (cbor_raw_match_fuel (n - 1)) pm0 elem v) (nondep_then parse_raw_data_item parse_raw_data_item) pm2_m map_ml2 map2_entries)
+          (cbor_raw_match_aux parse_raw_data_item (cbor_raw_match_fuel (n - 1)) pm2 x2 v2))
+        as (Trade.trade
+          (I.mixed_list_match (cbor_map_entry_vmatch_fuel (n - 1)) (nondep_then parse_raw_data_item parse_raw_data_item) pm2_m map_ml2 map2_entries)
+          (cbor_raw_match_aux parse_raw_data_item (cbor_raw_match_fuel (n - 1)) pm2 x2 v2));
+      intro
+        (trade
+          (cbor_raw_match_aux parse_raw_data_item (cbor_raw_match_fuel (n - 1)) pm2 x2 v2)
+          (cbor_raw_match_fuel n pm2 x2 v2))
+        #emp
+        fn _ {
+          cbor_raw_match_fuel_eq_succ n pm2 x2 v2;
+          rewrite (cbor_raw_match_aux parse_raw_data_item (cbor_raw_match_fuel (n - 1)) pm2 x2 v2)
+               as (cbor_raw_match_fuel n pm2 x2 v2)
+        };
+      Trade.trans
+        (I.mixed_list_match (cbor_map_entry_vmatch_fuel (n - 1)) (nondep_then parse_raw_data_item parse_raw_data_item) pm2_m map_ml2 map2_entries)
+        (cbor_raw_match_aux parse_raw_data_item (cbor_raw_match_fuel (n - 1)) pm2 x2 v2)
+        (cbor_raw_match_fuel n pm2 x2 v2);
+      let fwd = compare_cbor_raw_list_for_all_fuel (Ghost.hide (Ghost.reveal n - 1))
+                  #(check_equiv basic_data_model (option_nat_decrement_safe (NG.option_sz_v map_bound)))
+                  compare_rec_map f64
+                  map_ml2 map_ml1;
+      check_equiv_map_list_for_all_ext basic_data_model (option_nat_decrement_safe (NG.option_sz_v map_bound))
+        (list_sum (pair_sum raw_data_item_size raw_data_item_size) (Map?.v (Ghost.reveal v1)) + list_sum (pair_sum raw_data_item_size raw_data_item_size) (Map?.v (Ghost.reveal v2)))
+        (Ghost.reveal map2_entries) (Ghost.reveal map1_entries);
+      match fwd {
+        Some fwd_b -> {
+          if fwd_b {
+            let bwd = compare_cbor_raw_list_for_all_fuel (Ghost.hide (Ghost.reveal n - 1))
+                        #(check_equiv basic_data_model (option_nat_decrement_safe (NG.option_sz_v map_bound)))
+                        compare_rec_map f64
+                        map_ml1 map_ml2;
+            check_equiv_map_list_for_all_ext basic_data_model (option_nat_decrement_safe (NG.option_sz_v map_bound))
+              (list_sum (pair_sum raw_data_item_size raw_data_item_size) (Map?.v (Ghost.reveal v1)) + list_sum (pair_sum raw_data_item_size raw_data_item_size) (Map?.v (Ghost.reveal v2)))
+              (Ghost.reveal map1_entries) (Ghost.reveal map2_entries);
+            Trade.elim _ (cbor_raw_match_fuel n pm1 x1 v1);
+            Trade.elim _ (cbor_raw_match_fuel n pm2 x2 v2);
+            check_equiv_map_eq basic_data_model (NG.option_sz_v map_bound) (Ghost.reveal v1) (Ghost.reveal v2);
+            bwd
+          } else {
+            Trade.elim _ (cbor_raw_match_fuel n pm1 x1 v1);
+            Trade.elim _ (cbor_raw_match_fuel n pm2 x2 v2);
+            check_equiv_map_eq basic_data_model (NG.option_sz_v map_bound) (Ghost.reveal v1) (Ghost.reveal v2);
+            Some false
+          }
+        }
+        None -> {
+          Trade.elim _ (cbor_raw_match_fuel n pm1 x1 v1);
+          Trade.elim _ (cbor_raw_match_fuel n pm2 x2 v2);
+          check_equiv_map_eq basic_data_model (NG.option_sz_v map_bound) (Ghost.reveal v1) (Ghost.reveal v2);
+          None #bool
+        }
+      }
+    }
+  }
+}
+```
+
+#pop-options
