src/cbor/pulse/raw/everparse/CBOR.Pulse.Raw.EverParse.Nondet.Compare.Dispatch.fsti
@@ -1,0 +1,64 @@
+module CBOR.Pulse.Raw.EverParse.Nondet.Compare.Dispatch
+#lang-pulse
+include CBOR.Pulse.Raw.EverParse.Nondet.Compare.BasicTagged
+include CBOR.Pulse.Raw.EverParse.Nondet.Compare.BasicArray
+include CBOR.Pulse.Raw.EverParse.Nondet.Compare.BasicMap
+open CBOR.Spec.Util
+open CBOR.Spec.Raw.EverParse
+open CBOR.Pulse.Raw.EverParse.Type
+open CBOR.Pulse.Raw.EverParse.Match
+open CBOR.Pulse.Raw.EverParse.Match.Fuel
+open CBOR.Pulse.Raw.EverParse.Access
+open Pulse.Lib.Pervasives
+open Pulse.Lib.Trade
+
+module SZ = FStar.SizeT
+module Trade = Pulse.Lib.Trade.Util
+module U64 = FStar.UInt64
+module I16 = FStar.Int16
+module IT = LowParse.PulseParse.Iterator.Type
+module Spec = CBOR.Spec.API.Format
+module CompareBytes = CBOR.Pulse.Raw.Compare.Bytes
+module NG = CBOR.Pulse.Raw.EverParse.Nondet.Gen
+
+inline_for_extraction
+val compare_cbor_raw_basic_dispatch_body
+  (f64: squash SZ.fits_u64)
+  (map_bound: option SZ.t)
+  (n: Ghost.erased nat { Ghost.reveal n >= 1 })
+  (ih_tagged: compare_cbor_raw_basic_fuel_tagged_local_t n map_bound)
+  (ih_array: compare_cbor_raw_basic_fuel_array_local_t n map_bound)
+  (ih_map: compare_cbor_raw_basic_fuel_map_local_t n map_bound)
+  (x1 x2: cbor_raw)
+  (#pm1: perm) (#v1: Ghost.erased raw_data_item)
+  (#pm2: perm) (#v2: Ghost.erased raw_data_item)
+: stt (option bool)
+    (cbor_raw_match_fuel n pm1 x1 v1 **
+     cbor_raw_match_fuel n pm2 x2 v2 **
+     pure (raw_data_item_size v1 <= Ghost.reveal n /\
+           raw_data_item_size v2 <= Ghost.reveal n))
+    (fun res ->
+      cbor_raw_match_fuel n pm1 x1 v1 **
+      cbor_raw_match_fuel n pm2 x2 v2 **
+      pure (res == check_equiv basic_data_model (NG.option_sz_v map_bound) v1 v2))
+
+inline_for_extraction
+val compare_cbor_raw_basic_fuel_top
+  (f64: squash SZ.fits_u64)
+  (map_bound: option SZ.t)
+  (n: Ghost.erased nat)
+  (ih_tagged: compare_cbor_raw_basic_fuel_tagged_local_t n map_bound)
+  (ih_array: compare_cbor_raw_basic_fuel_array_local_t n map_bound)
+  (ih_map: compare_cbor_raw_basic_fuel_map_local_t n map_bound)
+  (x1 x2: cbor_raw)
+  (#pm1: perm) (#v1: Ghost.erased raw_data_item)
+  (#pm2: perm) (#v2: Ghost.erased raw_data_item)
+: stt (option bool)
+    (cbor_raw_match_fuel (Ghost.reveal n) pm1 x1 v1 **
+     cbor_raw_match_fuel (Ghost.reveal n) pm2 x2 v2 **
+     pure (raw_data_item_size v1 <= Ghost.reveal n /\
+           raw_data_item_size v2 <= Ghost.reveal n))
+    (fun res ->
+      cbor_raw_match_fuel (Ghost.reveal n) pm1 x1 v1 **
+      cbor_raw_match_fuel (Ghost.reveal n) pm2 x2 v2 **
+      pure (res == check_equiv basic_data_model (NG.option_sz_v map_bound) v1 v2))
