src/cbor/pulse/raw/everparse/CBOR.Pulse.Raw.EverParse.Nondet.Compare.Setoid.fsti
@@ -1,0 +1,46 @@
+module CBOR.Pulse.Raw.EverParse.Nondet.Compare.Setoid
+#lang-pulse
+include CBOR.Pulse.Raw.EverParse.Nondet.Compare.Base
+open CBOR.Spec.Util
+open CBOR.Spec.Raw.EverParse
+open CBOR.Pulse.Raw.EverParse.Type
+open CBOR.Pulse.Raw.EverParse.Match
+open CBOR.Pulse.Raw.EverParse.Match.Fuel
+open CBOR.Pulse.Raw.EverParse.MapEntry.Fuel
+open LowParse.PulseParse.Iterator
+open Pulse.Lib.Pervasives
+open Pulse.Lib.Trade
+
+module S = Pulse.Lib.Slice.Util
+module SZ = FStar.SizeT
+module R = Pulse.Lib.Reference
+module Trade = Pulse.Lib.Trade.Util
+module I = LowParse.PulseParse.Iterator
+module IT = LowParse.PulseParse.Iterator.Type
+
+inline_for_extraction
+val compare_cbor_raw_setoid_assoc_eq_fuel
+  (n: Ghost.erased nat { Ghost.reveal n >= 1 })
+  (#equiv: Ghost.erased (raw_data_item -> raw_data_item -> option bool))
+  (compare_impl: compare_cbor_raw_fn_fuel_t n equiv)
+  (f64: squash SZ.fits_u64)
+  (map_ml: IT.mixed_list (cbor_map_entry cbor_raw))
+  (#pm_map: perm)
+  (#map_entries: Ghost.erased (list (raw_data_item & raw_data_item)))
+  (xr: cbor_map_entry cbor_raw)
+  (#pm_xr: perm)
+  (#xr_pair: Ghost.erased (raw_data_item & raw_data_item))
+: stt (option bool)
+    (I.mixed_list_match (cbor_map_entry_vmatch_fuel n) (nondep_then parse_raw_data_item parse_raw_data_item)
+      pm_map map_ml map_entries **
+     cbor_map_entry_vmatch_fuel n pm_xr xr xr_pair **
+     pure (
+       list_sum (pair_sum raw_data_item_size raw_data_item_size) map_entries <= Ghost.reveal n /\
+       raw_data_item_size (fst (Ghost.reveal xr_pair)) <= Ghost.reveal n /\
+       raw_data_item_size (snd (Ghost.reveal xr_pair)) <= Ghost.reveal n
+     ))
+    (fun res ->
+      I.mixed_list_match (cbor_map_entry_vmatch_fuel n) (nondep_then parse_raw_data_item parse_raw_data_item)
+        pm_map map_ml map_entries **
+      cbor_map_entry_vmatch_fuel n pm_xr xr xr_pair **
+      pure (res == setoid_assoc_eq_with_overflow equiv equiv map_entries xr_pair))
